Adapt to ISA changes, and some minor cleanups

hardware/verilogLiftLib.sml
@@ -1,0 +1,69 @@
+structure verilogLiftLib =
+struct
+
+open combinSyntax fcpSyntax wordsSyntax stringSyntax;
+
+open verilogTypeTheory;
+
+open verilogTranslatorConfigLib;
+
+open verilogSyntax;
+
+local
+val (var_has_type_tm, mk_var_has_type, dest_var_has_type, is_var_has_type) = syntax_fns3 "verilogType" "var_has_type";
+in
+fun var_has_type_to_old_CONV tm =
+ if is_abs tm then
+   ABS_CONV var_has_type_to_old_CONV tm
+ else if is_var_has_type tm then let
+   val (_, _, ty) = dest_var_has_type tm
+ in
+   if is_VBool_t ty then (* BOOL *)
+     PURE_REWRITE_CONV [GSYM var_has_type_old_var_has_type_BOOL] tm
+   else if is_VArray_t ty then let
+     val is = dest_VArray_t ty
+     val len = length is
+   in
+     if len = 1 then (* WORD, TODO: assumes numerals in index position *) let
+       val dimindex_rw = is |> hd |> dest_numeral |> mk_numeric_type |> mk_dimindex |> EVAL |> SYM
+     in
+       PURE_REWRITE_CONV [dimindex_rw, GSYM var_has_type_old_var_has_type_WORD] tm
+     end else if len = 2 then (* WORD_ARRAY, TODO: does not work if index same... *) let
+       val dimword_rw = is |> hd |> dest_numeral |> Arbnumcore.log2 |> mk_numeric_type |> mk_dimword |> EVAL |> SYM
+       val dimindex_rw = is |> tl |> hd |> dest_numeral |> mk_numeric_type |> mk_dimindex |> EVAL |> SYM
+     in
+       PURE_REWRITE_CONV [dimword_rw, dimindex_rw, GSYM var_has_type_old_var_has_type_WORD_ARRAY] tm
+     end else
+       ALL_CONV tm
+   end else
+     ALL_CONV tm
+ end else if is_comb tm then
+   COMB_CONV var_has_type_to_old_CONV tm
+ else ALL_CONV tm
+end;
+
+val relM_backwards_tac =
+ CONV_TAC var_has_type_to_old_CONV \\
+
+ simp [var_has_type_old_def, var_has_value_def] \\
+
+ disch_then (MAP_EVERY (REPEAT_TCL CHOOSE_THEN ASSUME_TAC) o CONJUNCTS) \\
+
+ (fn g as (asl, _) => let
+     val hol_s = foldr (fn (assm, acc) => let
+                          val (lconj, rconj) = dest_conj assm
+                          val name = lconj |> lhs |> rand |> fromHOLstring
+                          val update = lookup name updates
+                          val rep = rconj |> rator |> rand
+                        in
+                          mk_comb(mk_comb (update, (mk_K_1 (rep, type_of rep))), acc)
+                        end)
+                       (mk_arb state_ty)
+                       asl
+  in
+    EXISTS_TAC hol_s g
+  end) \\
+
+ simp [];
+
+end
